Progress on incremental SHA2 in the new style

code/hash/Hacl.Impl.SHA2.fst
@@ -7,6 +7,8 @@ open FStar.HyperStack.ST
 open Spec.Lib.IntTypes
 open Spec.Lib.IntBuf
 open Spec.Lib.IntBuf.Lemmas
+open Spec.Lib.IntBuf.LoadStore
+
 open Spec.SHA2
 
 module ST = FStar.HyperStack.ST
@@ -23,6 +25,19 @@ inline_for_extraction let v = size_v
 inline_for_extraction let index (x:size_nat) = size x
 let op_String_Access #a #len m b = as_lseq #a #len b m
 
+(* Functions to add to the libraries *)
+val update_sub: #a:Type0 -> #len:size_nat -> #xlen:size_nat -> i:lbuffer a len -> start:size_t -> n:size_t{v start + v n <= len /\ v n == xlen} -> x:lbuffer a xlen ->
+  Stack unit
+    (requires (fun h -> live h i /\ live h x))
+    (ensures  (fun h0 _ h1 -> preserves_live h0 h1 /\ modifies1 i h0 h1
+                         /\ h1.[i] == Spec.Lib.IntSeq.update_sub #a #len h0.[i] (v start) (v n) h0.[x]))
+
+[@ Substitute]
+let update_sub #a #len #olen i start n x =
+  let i' = sub i start n in
+  copy i' n x
+
+
 
 (* Define algorithm parameters *)
 inline_for_extraction let size_hash_w : size_t = size Spec.size_hash_w
@@ -35,23 +50,10 @@ inline_for_extraction let max_input (p:Spec.parameters) = Spec.max_input p
 type block_w (p:Spec.parameters) = b:lbuffer (uint_t p.wt) 16
 type hash_w (p:Spec.parameters) = b:lbuffer (uint_t p.wt) Spec.size_hash_w
 type ws_w (p:Spec.parameters) = b:lbuffer (uint_t p.wt) p.kSize
+type iv_t (p:Spec.parameters) = b:lbuffer (uint_t p.wt) Spec.size_hash_w
 
 unfold type kTable (p:Spec.parameters) = b:lbuffer (uint_t p.wt) p.kSize
 unfold type wsTable (p:Spec.parameters) = b:lbuffer (uint_t p.wt) p.kSize
-
-
-(* Definition of constants *)
-inline_for_extraction val create_const_k: p:Spec.parameters -> StackInline (ws_w p)
-  (requires (fun h -> True))
-  (ensures (fun h0 r h1 -> creates1 r h0 h1 /\
-		                  preserves_live h0 h1 /\
-		                  modifies1 r h0 h1 /\
-		                  as_lseq r h1 == p.kTable))
-
-inline_for_extraction let create_const_k p =
-  admit()
-//  assert_norm(List.Tot.length p.kTable = 8);
-//  createL p.kTable
 
 
 #set-options "--max_fuel 0 --z3rlimit 50"
@@ -200,137 +202,158 @@ let compress p b kt s =
 (* Definition of the SHA2 state *)
 let len_block_t (p:Spec.parameters) = l:size_t{uint_v l < Spec.size_block p}
 
-noeq type state (p:Spec.parameters) =
+noeq type state (p:Spec.parameters) = {
+  hash:hash_w p;
+  const_iv: hash_w p;
+  const_k: ws_w p;
+}
+
+
+val state_invariant: h:mem -> p:Spec.parameters -> st:state p -> Type0
+let state_invariant h p st =
+    live h st.hash /\ live h st.const_k /\ live h st.const_iv
+  /\ disjoint st.hash st.const_iv /\ disjoint st.const_iv st.hash
+  /\ disjoint st.hash st.const_k /\ disjoint st.const_k st.hash
+  /\ disjoint st.const_iv st.const_k /\ disjoint st.const_k st.const_iv
+  /\ h.[st.const_iv] == p.h0
+  /\ h.[st.const_k] == p.kTable
+
+
+(* Definition of constants *)
+inline_for_extraction val create_const_iv: p:Spec.parameters -> StackInline (iv_t p)
+  (requires (fun h -> True))
+  (ensures (fun h0 r h1 -> creates1 r h0 h1 /\
+		                  preserves_live h0 h1 /\
+		                  modifies1 r h0 h1 /\
+		                  as_lseq r h1 == p.h0))
+
+inline_for_extraction let create_const_iv p = admit() // createL p.const_iv
+
+
+
+(* Definition of constants *)
+inline_for_extraction val create_const_k: p:Spec.parameters -> StackInline (ws_w p)
+  (requires (fun h -> True))
+  (ensures (fun h0 r h1 -> creates1 r h0 h1 /\
+		                  preserves_live h0 h1 /\
+		                  modifies1 r h0 h1 /\
+		                  as_lseq r h1 == p.kTable))
+
+inline_for_extraction let create_const_k p = admit() // createL p.kTable
+
+
+val mkstate: p:Spec.parameters ->
+  StackInline (st:state p)
+    (requires (fun h -> True))
+    (ensures  (fun h0 st h1 -> state_invariant h1 p st))
+
+let mkstate p =
   {
-    hash:lbuffer (uint_t p.wt) Spec.size_hash_w;
-    k:lbuffer (uint_t p.wt) p.kSize;
-    ws:lbuffer (uint_t p.wt) p.kSize;
-    blocks:lbuffer uint8 (2 * Spec.size_block_w);
-    len_block:lbuffer (uint_t p.wt) 1;
-    n:lbuffer (uint_t p.wt) 1;
-    tmp_block:lbuffer (uint_t p.wt) Spec.size_block_w;
+    hash = create (size Spec.size_hash_w) (nat_to_uint #p.wt 0);
+    const_iv = create_const_iv p;
+    const_k = create_const_k p;
   }
 
 
-let set_h0 (p:parameters) (hw:hash_w p) :
-  Stack unit
-        (requires (fun h -> live h hw))
-        (ensures  (fun h0 _ h1 -> preserves_live h0 h1 /\ modifies1 hw h0 h1
-                             /\ as_lseq hw h1 == p.h0)) =
-  hw.(size 0) <- p.h0.[0];
-  hw.(size 1) <- p.h0.[1];
-  hw.(size 2) <- p.h0.[2];
-  hw.(size 3) <- p.h0.[3];
-  hw.(size 4) <- p.h0.[4];
-  hw.(size 5) <- p.h0.[5];
-  hw.(size 6) <- p.h0.[6];
-  hw.(size 7) <- p.h0.[7];
-  admit()
-
 (* Definition of the initialization function for convenience *)
-assume val init: p:parameters ->
-  StackInline (state p)
-              (requires (fun h -> True))
-              (ensures  (fun h0 _ h1 -> True))
-// let init (p:parameters) :
-//   StackInline (state p)
-//               (requires (fun h -> True))
-//               (ensures  (fun h0 _ h1 -> True)) =
-//   let h0 : hash_w p = create #(uint_t p.wt) size_hash_w (nat_to_uint 0) in
-//   let ws0 : wsTable p = create #(uint_t p.wt) (uint_t p.kSize) (nat_to_uint 0) in
-//   let block0 : block_w p = create #(uint_t p.wt) size_block_w (nat_to_uint 0) in
-//   let tmp_block0 : block_w p = create #(uint_t p.wt) size_block_w (nat_to_uint 0) in
-//   set_h0 p h0;
-//   {hash = h0; ws = ws0; block = block0; len_block = size 0; n = size 0; tmp_block = tmp_block0}
+val init:
+    p:parameters
+  -> st:state p ->
+  Stack unit
+    (requires (fun h -> state_invariant h p st))
+    (ensures  (fun h0 _ h1 -> preserves_live h0 h1 /\ modifies1 st.hash h0 h1))
 
-(* Definition of the core compression function *)
-let update_block (p:parameters) (block:lbuffer uint8 (Spec.size_block p)) (st:state p)
-: Stack unit
-        (requires (fun h -> live h block))
-        (ensures  (fun h0 _ h1 -> preserves_live h0 h1 /\ modifies1 st.hash h0 h1)) =
-  Spec.Lib.IntBuf.LoadStore.uints_from_bytes_be st.tmp_block block;
-  ws p st.ws st.tmp_block;
-  let hash1 = st.hash in
-  shuffle p st.k st.ws st.hash;
-  map2 (size p.size_hash) (fun x y -> x +. y) st.hash hash1;
-  let n0 = st.n.(size 0) in
-  st.n.(size 0) <- n0 +. (size 1)
-
-(* Definition of the compression function iterated over multiple blocks *)
-let update_multi (p:parameters) (n:size_t{uint_v n * Spec.size_block p <= max_size_t}) (blocks:lbuffer uint8 (uint_v n * Spec.size_block p)) (st:state p)
-: Stack unit
-        (requires (fun h -> v (as_lseq st.n h).[0] + v n <= max_size_t))
-        (ensures  (fun h0 _ h1 -> preserves_live h0 h1 /\ modifies1 st.hash h0 h1)) =
-  let old_n = st.n in
-  let old_len_block = st.len_block in
-  iteri n
-    (fun i bl ->
-      // let h0 = ST.get () in
-      let sz_block = Spec.size_block p in
-      // FIXME let lseq_blocks = as_lseq blocks h0 in
-      // let lseq_block = LSeq.sub lseq_blocks FStar.Mul.(size_v sz_block * i) (size_v sz_block) in
-      let lseq_block = LSeq.create (Spec.size_block p) (nat_to_uint #p.wt 0) in
-      Spec.update_block p lseq_block)
-    (fun i bl ->
-      update_block p (sub blocks)) st
+let init p st =
+  copy st.hash size_hash_w st.const_iv
 
 
-(* Definition of the core compression function *)
-let update' (p:parameters) (len:size_t) (input:lbuffer uint8 (uint_v len)) (st:state p)
-: Stack unit
-        (requires (fun h -> True))
-        (ensures  (fun h0 _ h1 -> True)) =
-  let len_block = st.len_block.(size 0) in
-  if len_block +. len <. size_block p then begin
-    let block = sub #uint8 #(FStar.Mul.(2 * uint_v (size_block p))) #(uint_v len) st.blocks len_block len in
-    // copy #uint8 #(uint_v len) len input st.blocks;
-    let nv = len_block +. len in
-    // st.len_block.(size 0) <- nv;
-    () end
-  else begin
-    let prev_n = st.n in
-    // Fill the first part of the partial block and run update
-    let l1 = size_block p -. len_block in
-    let rem1 = sub input (size 0) l1 in
-    let block = sub st.blocks (size 0) (size_block p) in
-//    let block = update_sub block st.len_block l1 rem1 in
-//    let st = update_block p block st in
-//    let st = {st with n = prev_n + 1} in
-    () end
-  // else begin
-  //   let prev_n = st.n in
-  //   // Fill the first part of the partial block and run update
-  //   let l1 = size_block p - st.len_block in
-  //   let rem1 = sub input 0 l1 in
-  //   let block = sub st.blocks 0 (size_block p) in
-  //   let block = update_sub block st.len_block l1 rem1 in
-  //   let st = update_block p block st in
-  //   let st = {st with n = prev_n + 1} in
-  //   // Handle full blocks in the rest of the input data
-  //   let l2 : size_nat = len - l1 in
-  //   let rem2 = sub input l1 l2 in
-  //   let n : size_nat = l2 / size_block p in
-  //   let r : size_nat = l2 % size_block p in
-  //   let blocks = sub #uint8 #l2 rem2 0 (n * (size_block p)) in
-  //   let st = update_multi p n blocks st in
-  //   // Handle the remainder of the input
-  //   let rem3 = sub #uint8 #l2 rem2 (n * (size_block p)) r in
-  //   let pblock = update_sub st.blocks 0 r rem3 in
-  //   {st with blocks = pblock; len_block = r}
-  // end
+val update_block: p:parameters -> st:state p -> block:lbuffer uint8 (Spec.size_block p) ->
+  Stack unit
+  (requires (fun h -> live h st.hash /\ live h block))
+  (ensures  (fun h0 _ h1 -> preserves_live h0 h1 /\ modifies1 st.hash h0 h1))
 
-(* Definition of the finalization function *)
-let finish' (p:parameters) (st:state p{st.n + number_blocks_padding_single p st.len_block <= max_size_t}) : lbytes p.size_hash =
-  let pblock = sub st.blocks 0 st.len_block in
-  let blocks = pad p st.n st.len_block pblock in
-  assert(st.n + number_blocks_padding_single p st.len_block <= max_size_t);
-  let st = update_multi p (number_blocks_padding_single p st.len_block) blocks st in
-  let hash_final = uints_to_bytes_be st.hash in
-  let h = slice hash_final 0 p.size_hash in
-  h
+let update_block p st block =
+  (**) let h0 = ST.get () in
+  alloc1 #h0 size_block_w (u8 0) st.hash
+  (fun h0 -> (fun _ sv -> True))
+  (fun bw ->
+    uints_from_bytes_be bw block;
+    compress p bw st.const_k st.hash
+  )
 
-(* Definition of the SHA2 ontime function based on incremental calls *)
-let hash' (p:parameters) (len:size_nat{len < max_input p}) (input:lbytes len) : lbytes p.size_hash =
-  let st = init p in
-  let st = update' p len input st in
-  finish' p st
+
+val update_multi_iteration:
+    p:Spec.parameters
+  -> st:state p
+  -> n_prev:size_t
+  -> n:size_t{(v n + v n_prev) * Spec.size_block p <= max_size_t}
+  -> b:lbuffer uint8 (v n * Spec.size_block p)
+  -> i:size_t{v i + 1 <= v n} ->
+  Stack unit
+    (requires (fun h -> state_invariant h p st
+                   /\ live h b /\ disjoint st.hash b /\ disjoint b st.hash))
+    (ensures  (fun h0 _ h1 -> preserves_live h0 h1 /\ modifies1 st.hash h0 h1))
+
+[@ Substitute ]
+let update_multi_iteration p st n_prev n b i =
+  let block = sub b (i *. (size (Spec.size_block p))) (size (Spec.size_block p)) in
+  update_block p st block
+
+
+val update_multi:
+    p: Spec.parameters
+  -> st: state p
+  -> n_prev: size_t
+  -> n: size_t{(v n + v n_prev) * Spec.size_block p <= max_size_t}
+  -> b: lbuffer uint8 (size_v n * Spec.size_block p) ->
+   Stack unit
+     (requires (fun h -> state_invariant h p st
+                    /\ live h b /\ disjoint st.hash b /\ disjoint b st.hash))
+     (ensures  (fun h0 _ h1 -> preserves_live h0 h1 /\ modifies1 st.hash h0 h1))
+
+let update_multi p st n_prev n b =
+  (**) let h0 = ST.get () in
+  loop #h0 n st.hash
+  (fun hi -> (fun i s -> s))
+  (fun i -> update_multi_iteration p st n_prev n b i)
+
+
+val finish:
+    p: Spec.parameters
+  -> output: lbuffer uint8 (Spec.size_hash p)
+  -> st: state p ->
+  Stack unit
+    (requires (fun h -> state_invariant h p st
+                   /\ live h output /\ disjoint output st.hash /\ disjoint st.hash output))
+    (ensures  (fun h0 _ h1 -> preserves_live h0 h1 /\ modifies1 output h0 h1))
+
+let finish p output s =
+  (**) let h0 = ST.get () in
+  alloc1 #h0 (size 32) (u8 0) output
+  (fun h -> (fun _ r -> True))
+  (fun full ->
+    uints_to_bytes_le full s.hash;
+    update_sub output (size 0) (size (size_hash p)) full)
+
+
+val sha2:
+    #vlen: size_nat
+  -> p:Spec.parameters
+  -> output: lbuffer uint8 (Spec.size_hash p)
+  -> input: lbuffer uint8 vlen
+  -> len: size_t{v len <= max_input p /\ v len = vlen} ->
+  Stack unit
+    (requires (fun h -> live h output /\ live h input
+                   /\ disjoint output input /\ disjoint input output))
+    (ensures  (fun h0 _ h1 -> preserves_live h0 h1 /\ modifies1 output h0 h1))
+
+let sha2 #vlen p output input len =
+  let rem = len %. (size (Spec.size_block p)) in
+  let nblocks = len /. (size (Spec.size_block p)) in
+  let blocks = sub #uint8 #vlen #(v nblocks * (Spec.size_block p)) input (size 0) (nblocks *. (size (Spec.size_block p))) in
+  let last = sub input (nblocks *. (size (Spec.size_block p))) rem in
+  let st = mkstate p in
+  init p st;
+  update_multi p st (size 0) nblocks input;
+  update_last p st len last rem;
+  finish p output st
